@prefix brick: <https://brickschema.org/schema/Brick#> .
@prefix csvw: <http://www.w3.org/ns/csvw#> .
@prefix dc: <http://purl.org/dc/elements/1.1/> .
@prefix dcam: <http://purl.org/dc/dcam/> .
@prefix dcat: <http://www.w3.org/ns/dcat#> .
@prefix dcmitype: <http://purl.org/dc/dcmitype/> .
@prefix dcterms: <http://purl.org/dc/terms/> .
@prefix doap: <http://usefulinc.com/ns/doap#> .
@prefix foaf: <http://xmlns.com/foaf/0.1/> .
@prefix geo: <http://www.opengis.net/ont/geosparql#> .
@prefix mds: <https://cwrusdle.bitbucket.io/mds#> .
@prefix odrl: <http://www.w3.org/ns/odrl/2/> .
@prefix org: <http://www.w3.org/ns/org#> .
@prefix owl: <http://www.w3.org/2002/07/owl#> .
@prefix pmdco: <https://w3id.org/pmd/co/> .
@prefix prof: <http://www.w3.org/ns/dx/prof/> .
@prefix prov: <http://www.w3.org/ns/prov#> .
@prefix qb: <http://purl.org/linked-data/cube#> .
@prefix qudt: <http://qudt.org/2.1/vocab/unit/> .
@prefix rdf: <http://www.w3.org/1999/02/22-rdf-syntax-ns#> .
@prefix rdfs: <http://www.w3.org/2000/01/rdf-schema#> .
@prefix schema: <https://schema.org/> .
@prefix sh: <http://www.w3.org/ns/shacl#> .
@prefix skos: <http://www.w3.org/2004/02/skos/core#> .
@prefix sosa: <http://www.w3.org/ns/sosa/> .
@prefix ssn: <http://www.w3.org/ns/ssn/> .
@prefix time: <http://www.w3.org/2006/time#> .
@prefix vann: <http://purl.org/vocab/vann/> .
@prefix void: <http://rdfs.org/ns/void#> .
@prefix wgs: <https://www.w3.org/2003/01/geo/wgs84_pos#> .
@prefix xml: <http://www.w3.org/XML/1998/namespace> .
@prefix xsd: <http://www.w3.org/2001/XMLSchema#> .

dcterms:isPartOf a owl:ObjectProperty ;
    rdfs:domain mds:CellReferenceConstant,
        mds:FacilityAmbientTemperature,
        mds:FlashWaitTime,
        mds:LoadPulseLength,
        mds:ModuleLoadVoltage,
        mds:NumberOfCellsPerString,
        mds:NumberStrings,
        mds:SimulatorMeasurementType,
        mds:SunIntensity,
        mds:VoltageTemperatureCoefficient,
        mds:WaferDopingType ;
    rdfs:range mds:CurrentVoltageRecipe .


mds:CurrentVoltageDataFilePath a owl:Class ;
    rdfs:subClassOf mds:FilePath ;
    skos:definition "The file path of a dataset generated by a current voltage process" .

mds:CurrentVoltageRecipeAuthor a owl:Class ;
    rdfs:subClassOf mds:Recipe ;
    skos:definition "The author of a recipe for a current voltage process" .

mds:CurrentVoltageRecipeCreatedDate a owl:Class ;
    rdfs:subClassOf mds:Recipe ;
    skos:definition "The creation date for a current voltage process recipe" .

mds:CurrentVoltageRecipeFilePath a owl:Class ;
    rdfs:subClassOf mds:Recipe ;
    skos:definition "The file path for a current voltage process recipe" .

mds:CurrentVoltageRecipeID a owl:Class ;
    rdfs:subClassOf mds:RecipeID ;
    skos:definition "The identification number for a current voltage recipe" .

mds:CurrentVoltageResultsTimestamp a owl:Class ;
    rdfs:subClassOf mds:Date ;
    skos:definition "The datetime when a current voltage process was executed" .

mds:LoadVoltage a owl:Class ;
    rdfs:subClassOf mds:Tool ;
    skos:definition "The standard testing condition load voltage of a sample being measured" .


mds:SimulatorToolModel a owl:Class ;
    rdfs:subClassOf mds:ToolModel ;
    skos:definition "The model of the solar simulator, i.e. FMT-350" .

mds:SimulatorToolSerialNo a owl:Class ;
    rdfs:subClassOf mds:ToolSerialNo ;
    skos:definition "The serial number of a solar simulator" .

mds:SolarSimulatorID a owl:Class ;
    rdfs:subClassOf mds:ToolID ;
    skos:definition "The identification number of a solar simulator" .

mds:SolarSimulatorManufacturer a owl:Class ;
    rdfs:subClassOf mds:ToolManufacturer ;
    skos:definition "The manufacturer of a solar simulator, i.e. 'Sinton Instruments'" .

mds:SolarSimulatorName a owl:Class ;
    rdfs:subClassOf mds:ToolName ;
    skos:definition "The name of a solar simulator, i.e. 'Lab 1 Simulator'" .


mds:CurrentVoltageStepSize a owl:Class ;
    rdfs:subClassOf mds:Tool ;
    skos:definition "The step size of the voltage for a current voltage process" .


mds:SampleCellArea a owl:Class ;
    rdfs:subClassOf mds:Sample ;
    skos:definition "Area of an invididual cell within a module that a current voltage process is being performed on" .

mds:SampleTotalArea a owl:Class ;
    rdfs:subClassOf mds:Sample ;
    skos:definition "Total area of the module that a current voltage process is being performed on" .

mds:SimulatorSpatialUniformity a owl:Class ;
    rdfs:subClassOf mds:Tool ;
    skos:definition "The spational uniformity of a simulator" .


mds:CellEfficiency a owl:Class ;
    rdfs:subClassOf mds:Result ;
    skos:definition "The cell efficiency measured by a current voltage process" .

mds:CellReferenceConstant a owl:Class ;
    rdfs:subClassOf mds:Tool ;
    skos:definition "A calibration setting that deteremines the irradiance level of a light source, typically determined by a reference cell" .

mds:CurrentAtMaxPower a owl:Class ;
    rdfs:subClassOf mds:Result ;
    skos:definition "The current at max power measured by a current voltage process" .

mds:CurrentVoltageAnalysis a owl:Class ;
    rdfs:subClassOf mds:Analysis ;
    skos:definition "The analysis method used on a raw dataset generated by a current voltage process" .

mds:CurrentVoltageData a owl:Class ;
    rdfs:subClassOf mds:Result ;
    skos:definition "The raw current voltage data generated by a current voltage process" .

mds:CurrentVoltageResults a owl:Class ;
    rdfs:subClassOf mds:Result ;
    skos:definition "The parameters that resulted from the current voltage process " .

mds:CurrentVoltageSample a owl:Class ;
    rdfs:subClassOf mds:Sample ;
    skos:definition "A sample used in a current voltage process" .

mds:FacilityAmbientTemperature a owl:Class ;
    rdfs:subClassOf mds:Recipe ;
    skos:definition "The ambient temperature of the room that a current voltage process is being performed in" .

mds:FillFactor a owl:Class ;
    rdfs:subClassOf mds:Result ;
    skos:definition "The fill factor measured by a current voltage process" .

mds:FlashWaitTime a owl:Class ;
    rdfs:subClassOf mds:Recipe ;
    skos:definition "The amount of time between flash pulses" .

mds:LoadPulseLength a owl:Class ;
    rdfs:subClassOf mds:Recipe ;
    skos:definition "The amount of time data is acquired during flash pulses" .

mds:MaximumPowerPoint a owl:Class ;
    rdfs:subClassOf mds:Result ;
    skos:definition "The maximum power point measured by a current voltage process" .

mds:OpenCircuitVoltage a owl:Class ;
    rdfs:subClassOf mds:Result ;
    skos:definition "The open circuit voltage measured by a current voltage process" .

mds:SampleResistivity a owl:Class ;
    rdfs:subClassOf mds:Sample ;
    skos:definition "Resisitivity of the sample that a current voltage is being performed on" .

mds:SaturationCurrentDensity a owl:Class ;
    rdfs:subClassOf mds:Result ;
    skos:definition "The saturation current density measured by a current voltage process" .

mds:SeriesResistance a owl:Class ;
    rdfs:subClassOf mds:Result ;
    skos:definition "The series resistance measured by a current voltage process" .

mds:ShortCircuitCurrent a owl:Class ;
    rdfs:subClassOf mds:Result ;
    skos:definition "The short circuit current measured by a current voltage process" .

mds:ShuntResistance a owl:Class ;
    rdfs:subClassOf mds:Result ;
    skos:definition "The shunt resistance measured by a current voltage process" .

mds:SimulatorCurrentRange a owl:Class ;
    rdfs:subClassOf mds:Recipe ;
    skos:definition "The working range of the current of a simulator" .

mds:SimulatorIntensityRange a owl:Class ;
    rdfs:subClassOf mds:Recipe ;
    skos:definition "The working range of the intensity of a simulator" .

mds:SimulatorVoltageRange a owl:Class ;
    rdfs:subClassOf mds:Recipe ;
    skos:definition "The working range of the voltage of a simulator" .

mds:SolarSimulator a owl:Class ;
    rdfs:subClassOf mds:Tool ;
    skos:definition "A tool used to simulate the environment of a sun for a PV module, to perform a current voltage measurement" .

mds:SunIntensity a owl:Class ;
    rdfs:subClassOf mds:Tool ;
    skos:definition "The established intensity of a current voltage process" .

mds:VoltageAtMaxPower a owl:Class ;
    rdfs:subClassOf mds:Result ;
    skos:definition "The voltage at max power measured by a current voltage process" .

mds:NumberOfCellsPerString a owl:Class ;
    rdfs:subClassOf mds:Tool ;
    skos:definition "Number of cells in a group of solar panels connected in series in a module" .

mds:NumberStrings a owl:Class ;
    rdfs:subClassOf mds:Tool ;
    skos:definition "Number of groups of solar panels connected in series in a module" .

mds:SimulatorMeasurementType a owl:Class ;
    rdfs:subClassOf mds:Tool ;
    skos:definition "Type of measurement a simulator is performing" .

mds:VoltageTemperatureCoefficient a owl:Class ;
    rdfs:subClassOf mds:Sample ;
    skos:definition "The amount a cell's output voltage changes due to temperature" .

mds:WaferDopingType a owl:Class ;
    rdfs:subClassOf mds:Sample ;
    skos:definition "Doping type of the wafer that a current voltage process is being performed on" .

mds:CurrentVoltageRecipe a owl:Class ;
    rdfs:subClassOf mds:Recipe ;
    skos:broader mds:Recipe ;
    skos:definition "A recipe describing the settings for a current voltage process" .

mds: a owl:Ontology ;
    dcterms:creator "Brent Thompson",
        "Jarod Kaltenbaugh",
        "Kristopher O. Davis",
        "Quynh Tran",
        "Roger H. French" ;
    dcterms:description "Ontology describing a generic current voltage measurement process" ;
    dcterms:title "" ;
    owl:imports <http://purl.org/dc/dcam/> ,
        <http://purl.org/dc/dcmitype/> ,
        <http://purl.org/dc/elements/1.1/> ,
        <http://purl.org/dc/terms/> ,
        <http://purl.org/linked-data/cube#> ,
        <http://purl.org/vocab/vann/> ,
        <http://qudt.org/2.1/vocab/unit/> ,
        <http://rdfs.org/ns/void#> ,
        <http://usefulinc.com/ns/doap#> ,
        <http://www.opengis.net/ont/geosparql#> ,
        <http://www.w3.org/1999/02/22-rdf-syntax-ns#> ,
        <http://www.w3.org/2000/01/rdf-schema#> ,
        <http://www.w3.org/2001/XMLSchema#> ,
        <http://www.w3.org/2002/07/owl#> ,
        <http://www.w3.org/2004/02/skos/core#> ,
        <http://www.w3.org/2006/time#> ,
        <http://www.w3.org/XML/1998/namespace> ,
        <http://www.w3.org/ns/csvw#> ,
        <http://www.w3.org/ns/dcat#> ,
        <http://www.w3.org/ns/dx/prof/> ,
        <http://www.w3.org/ns/odrl/2/> ,
        <http://www.w3.org/ns/org#> ,
        <http://www.w3.org/ns/prov#> ,
        <http://www.w3.org/ns/shacl#> ,
        <http://www.w3.org/ns/sosa/> ,
        <http://www.w3.org/ns/ssn/> ,
        <http://xmlns.com/foaf/0.1/> ,
        <https://brickschema.org/schema/Brick#> ,
        <https://cwrusdle.bitbucket.io/mds#> ,
        <https://schema.org/> ,
        <https://w3id.org/pmd/co/> ,
        <https://www.w3.org/2003/01/geo/wgs84_pos#>  ;
    dcterms:license <https://creativecommons.org/licenses/by-sa/4.0/> ;
    owl:versionInfo "0.3.0.0" .

